Finish VM

theories/vm/Semantics.v
@@ -1,5 +1,47 @@
 From Books Require Import Tactics.
 From Books.vm Require Import Syntax.
-From Stdlib Require Import List.
+From Stdlib Require Import List NArith.
 Import ListNotations.
 Open Scope N_scope.
+
+Inductive step (p : program) : stack -> pc -> stack -> pc -> Prop :=
+| SConst : forall n st pc,
+    p pc = Some (Const n) ->
+    step p st pc (n :: st) (pc + 1)
+| SPop : forall n st pc,
+    p pc = Some Pop ->
+    step p (n :: st) pc st (pc + 1)
+| SPlus : forall n1 n2 st pc,
+    p pc = Some Plus ->
+    step p (n1 :: n2 :: st) pc (n1 + n2 :: st) (pc + 1)
+| SJmp : forall pc' st pc,
+    p pc = Some (Jmp pc') ->
+    step p st pc st pc'
+| SJnzT : forall n pc' st pc,
+    p pc = Some (Jnz pc') ->
+    0 < n ->
+    step p (n :: st) pc (n :: st) pc'
+| SJnzF : forall pc' st pc,
+    p pc = Some (Jnz pc') ->
+    step p (0 :: st) pc (0 :: st) (pc + 1).
+
+Hint Constructors step : core.
+
+Ltac solve_ppc :=
+  match goal with
+  | [H: ?p ?pc = Some ?x, H0: ?p ?pc = Some ?y |- _] => rewrite H in H0; inv H0
+  end.
+
+Theorem step_deterministic :
+  forall p st pc st1' pc1' st2' pc2',
+    step p st pc st1' pc1' ->
+    step p st pc st2' pc2' ->
+    st1' = st2' /\ pc1' = pc2'.
+Proof.
+  intros. assert (p pc = None \/ exists instr, p pc = Some instr). {
+    destruct (p pc). right. now exists i. now left.
+  } destruct H1. exfalso. inv H; rewrite H1 in H2; discriminate.
+  destruct H1 as (I & PPCI). revert st1' pc1' st2' pc2' p pc st PPCI H H0.
+  destruct I; intros.
+  all: inv H; solve_ppc; inv H0; solve_ppc; easy.
+Qed.
