theories/vm/Syntax.v
@@ -1,4 +1,5 @@
-From Stdlib Require Import NArith.
+From Stdlib Require Import NArith List.
+Open Scope N_scope.
 
 Definition stack : Type := list N.
 Definition pc : Type := N.
@@ -6,7 +7,7 @@ Definition pc : Type := N.
 Inductive instr : Type :=
   | Const (n : N)
   | Pop
-  | Add
+  | Plus
   | Jmp (pos : pc)
   | Jnz (pos : pc).
 
@@ -14,4 +15,13 @@ Definition stmt_eqdec (st1 st2 : instr) : {st1=st2} + {st1<>st2}.
   repeat decide equality.
 Defined.
 
-Definition program : Type := list instr.
+Definition program : Type := pc -> option instr.
+
+Definition plist : Type := list instr.
+Definition program_of_plist (pl : plist) : program :=
+  snd (fold_left (
+    fun a i =>
+      match a with
+      | (pc, prog) => (pc + 1, fun pc' => if pc' =? pc then Some i else prog pc')
+      end
+  ) pl (0, (fun _ => None))).
