theories/vm/FInterp.v
@@ -1,0 +1,60 @@
+From Books.vm Require Import Syntax Semantics.
+From Books Require Import Tactics.
+From Stdlib Require Import NArith List Lia.
+Import ListNotations.
+
+Definition fstep (p : program) (st : stack) (pcnt : pc) : option (stack * pc) :=
+  match p pcnt with
+  | Some (Const n) => Some (n :: st, pcnt + 1)
+  | Some Pop =>
+      match st with
+      | [] => None
+      | h :: t => Some (t, pcnt + 1)
+      end
+  | Some Plus =>
+      match st with
+      | n :: m :: t => Some (n + m :: t, pcnt + 1)
+      | _ => None
+      end
+  | Some (Jmp pcnt') => Some (st, pcnt')
+  | Some (Jnz pcnt') =>
+      match st with
+      | x :: t => Some (st, if x =? 0 then pcnt + 1 else pcnt')
+      | _ => None
+      end
+  | _ => None
+  end.
+
+Section FInterpCorrectness.
+
+Theorem fstep_sound :
+  forall p st pc st' pc',
+    fstep p st pc = Some (st', pc') ->
+    step p st pc st' pc'.
+Proof.
+  intros. assert (p pc = None \/ exists instr, p pc = Some instr). {
+    destruct (p pc). right. now exists i. now left.
+  } destruct H0. unfold fstep in H. rewrite H0 in H. discriminate.
+  destruct H0 as (I & PPCI). destruct I.
+  all: unfold fstep in H; rewrite PPCI in H; inv H.
+  - (* Const *) now constructor.
+  - (* Pop *) destruct st; inv H1. now constructor.
+  - (* Plus *) destruct st; inv H1; destruct st; inv H0. now constructor.
+  - (* Jmp *) now constructor.
+  - (* Jnz *) destruct st; inv H1. destruct (n =? 0) eqn:E.
+      replace n with 0 in *. eauto. apply N.eqb_eq in E. now subst.
+      apply SJnzT. assumption. apply N.eqb_neq in E. lia.
+Qed.
+
+Theorem fstep_complete :
+  forall p st pc st' pc',
+    step p st pc st' pc' ->
+    fstep p st pc = Some (st', pc').
+Proof.
+  intros. induction H; unfold fstep; rewrite H; clear H; auto.
+  destruct (n =? 0) eqn:E.
+    apply N.eqb_eq in E. lia.
+    reflexivity.
+Qed.
+
+End FInterpCorrectness.
